CryptoPrims/CryptoTests.lean
@@ -12,19 +12,20 @@ attribute [simp] Fin.foldr_succ
   ["0"] : (Public)  by {
       unfold sideConditions
       simp
+      grind
   }
 
 #tc ENC_FUNC := · ; · ; · ; · ⊢
     Λβ betaK .
     Λβ betaM .
     Λ tau .
-    let k = (⟨"genKey"⟩ (["0"], ["0"]) : Data betaK) in
+    let k = (⟨"genKey"⟩ (["0"], ["0"]) : Data betaK ) in
     let L = alloc (λ (null : Public) : (tau + unit) => ı2 ()) in
     let enc' = (corr_case betaK in
                 (if corr ( betaK )
                   then (λ (x : (Public * Public)) : Public => ⟨"enc"⟩ (π1 x, π2 x))
                   else
-                    λ (x : (Data betaK * tau)) : Public =>
+                    λ (x : (Data betaK * tau )) : Public =>
                     let c = ⟨"rand"⟩ (zero ((π2 x) : Data betaM), ["0"]) in
                     let L_old = (! L) in
                     let sc = (L := (λ (y : Public) : (tau + unit) => if ⟨"eq"⟩(y, c) then ı1 (π2 x) else (L_old [y]))) in
@@ -46,9 +47,7 @@ attribute [simp] Fin.foldr_succ
       unfold sideConditions
       simp
       grind
-
     }
-
 
 -- Bonus points: make it a record
 
